test: new frontend

tests/lean/run/sharecommon.lean
@@ -5,35 +5,35 @@ def check (b : Bool) : ShareCommonT IO Unit :=
 unless b $ throw $ IO.userError "check failed"
 
 unsafe def tst1 : ShareCommonT IO Unit := do
-let x := [1];
-let y := [0].map (fun x => x + 1);
-check $ ptrAddrUnsafe x != ptrAddrUnsafe y;
-let x ← shareCommonM x;
-let y ← shareCommonM y;
-check $ ptrAddrUnsafe x == ptrAddrUnsafe y;
-let z ← shareCommonM [2];
-let x ← shareCommonM x;
-check $ ptrAddrUnsafe x == ptrAddrUnsafe y;
-check $ ptrAddrUnsafe x != ptrAddrUnsafe z;
-IO.println x;
-IO.println y;
+let x := [1]
+let y := [0].map (fun x => x + 1)
+check $ ptrAddrUnsafe x != ptrAddrUnsafe y
+let x ← shareCommonM x
+let y ← shareCommonM y
+check $ ptrAddrUnsafe x == ptrAddrUnsafe y
+let z ← shareCommonM [2]
+let x ← shareCommonM x
+check $ ptrAddrUnsafe x == ptrAddrUnsafe y
+check $ ptrAddrUnsafe x != ptrAddrUnsafe z
+IO.println x
+IO.println y
 IO.println z
 
 #eval tst1.run
 
 unsafe def tst2 : ShareCommonT IO Unit := do
-let x := [1, 2];
-let y := [0, 1].map (fun x => x + 1);
-check $ ptrAddrUnsafe x != ptrAddrUnsafe y;
-let x ← shareCommonM x;
-let y ← shareCommonM y;
-check $ ptrAddrUnsafe x == ptrAddrUnsafe y;
-let z ← shareCommonM [2];
-let x ← shareCommonM x;
-check $ ptrAddrUnsafe x == ptrAddrUnsafe y;
-check $ ptrAddrUnsafe x != ptrAddrUnsafe z;
-IO.println x;
-IO.println y;
+let x := [1, 2]
+let y := [0, 1].map (fun x => x + 1)
+check $ ptrAddrUnsafe x != ptrAddrUnsafe y
+let x ← shareCommonM x
+let y ← shareCommonM y
+check $ ptrAddrUnsafe x == ptrAddrUnsafe y
+let z ← shareCommonM [2]
+let x ← shareCommonM x
+check $ ptrAddrUnsafe x == ptrAddrUnsafe y
+check $ ptrAddrUnsafe x != ptrAddrUnsafe z
+IO.println x
+IO.println y
 IO.println z
 
 #eval tst2.run
@@ -47,38 +47,38 @@ structure Foo :=
 @[noinline] def mkFoo2 (x : Nat) (z : Bool) : Foo := { x := x, y := true, z := z }
 
 unsafe def tst3 : ShareCommonT IO Unit := do
-let o1 := mkFoo1 10 true;
-let o2 := mkFoo2 10 true;
-let o3 := mkFoo2 10 false;
-check $ ptrAddrUnsafe o1 != ptrAddrUnsafe o2;
-check $ ptrAddrUnsafe o1 != ptrAddrUnsafe o3;
-let o1 ← shareCommonM o1;
-let o2 ← shareCommonM o2;
-let o3 ← shareCommonM o3;
+let o1 := mkFoo1 10 true
+let o2 := mkFoo2 10 true
+let o3 := mkFoo2 10 false
+check $ ptrAddrUnsafe o1 != ptrAddrUnsafe o2
+check $ ptrAddrUnsafe o1 != ptrAddrUnsafe o3
+let o1 ← shareCommonM o1
+let o2 ← shareCommonM o2
+let o3 ← shareCommonM o3
 check $
   o1.x == 10 && o1.y == true &&
   o1.z == true && o3.z == false &&
   ptrAddrUnsafe o1 == ptrAddrUnsafe o2 &&
-  ptrAddrUnsafe o1 != ptrAddrUnsafe o3;
-IO.println o1.x;
+  ptrAddrUnsafe o1 != ptrAddrUnsafe o3
+IO.println o1.x
 pure ()
 
 #eval tst3.run
 
 unsafe def tst4 : ShareCommonT IO Unit := do
-let x := ["hello"];
-let y := ["ello"].map (fun x => "h" ++ x);
-check $ ptrAddrUnsafe x != ptrAddrUnsafe y;
-let x ← shareCommonM x;
-let y ← shareCommonM y;
-check $ ptrAddrUnsafe x == ptrAddrUnsafe y;
-let z ← shareCommonM ["world"];
-let x ← shareCommonM x;
+let x := ["hello"]
+let y := ["ello"].map (fun x => "h" ++ x)
+check $ ptrAddrUnsafe x != ptrAddrUnsafe y
+let x ← shareCommonM x
+let y ← shareCommonM y
+check $ ptrAddrUnsafe x == ptrAddrUnsafe y
+let z ← shareCommonM ["world"]
+let x ← shareCommonM x
 check $
   ptrAddrUnsafe x == ptrAddrUnsafe y &&
-  ptrAddrUnsafe x != ptrAddrUnsafe z;
-IO.println x;
-IO.println y;
+  ptrAddrUnsafe x != ptrAddrUnsafe z
+IO.println x
+IO.println y
 IO.println z
 
 #eval tst4.run
@@ -91,57 +91,57 @@ IO.println z
 mkArray1 x
 
 unsafe def tst5 : ShareCommonT IO Unit := do
-let a := mkArray1 3;
-let b := mkArray2 3;
-let c := mkArray2 4;
-IO.println a;
-IO.println b;
-IO.println c;
+let a := mkArray1 3
+let b := mkArray2 3
+let c := mkArray2 4
+IO.println a
+IO.println b
+IO.println c
 check $
   ptrAddrUnsafe a != ptrAddrUnsafe b &&
   ptrAddrUnsafe a != ptrAddrUnsafe c &&
-  ptrAddrUnsafe (a.get! 0) != ptrAddrUnsafe (a.get! 1) &&
-  ptrAddrUnsafe (a.get! 0) != ptrAddrUnsafe (a.get! 2) &&
-  ptrAddrUnsafe (b.get! 0) != ptrAddrUnsafe (b.get! 1) &&
-  ptrAddrUnsafe (c.get! 0) != ptrAddrUnsafe (c.get! 1);
-let a ← shareCommonM a;
-let b ← shareCommonM b;
-let c ← shareCommonM c;
+  ptrAddrUnsafe a[0] != ptrAddrUnsafe a[1] &&
+  ptrAddrUnsafe a[0] != ptrAddrUnsafe a[2] &&
+  ptrAddrUnsafe b[0] != ptrAddrUnsafe b[1] &&
+  ptrAddrUnsafe c[0] != ptrAddrUnsafe c[1]
+let a ← shareCommonM a
+let b ← shareCommonM b
+let c ← shareCommonM c
 check $
   ptrAddrUnsafe a == ptrAddrUnsafe b &&
   ptrAddrUnsafe a != ptrAddrUnsafe c &&
-  ptrAddrUnsafe (a.get! 0) == ptrAddrUnsafe (a.get! 1) &&
-  ptrAddrUnsafe (a.get! 0) != ptrAddrUnsafe (a.get! 2) &&
-  ptrAddrUnsafe (b.get! 0) == ptrAddrUnsafe (b.get! 1) &&
-  ptrAddrUnsafe (c.get! 0) == ptrAddrUnsafe (c.get! 1);
+  ptrAddrUnsafe a[0] == ptrAddrUnsafe a[1] &&
+  ptrAddrUnsafe a[0] != ptrAddrUnsafe a[2] &&
+  ptrAddrUnsafe b[0] == ptrAddrUnsafe b[1] &&
+  ptrAddrUnsafe c[0] == ptrAddrUnsafe c[1]
 pure ()
 
 #eval tst5.run
 
 @[noinline] def mkByteArray1 (x : Nat) : ByteArray :=
-let r := ByteArray.empty;
-let r := r.push x.toUInt8;
-let r := r.push (x+1).toUInt8;
-let r := r.push (x+2).toUInt8;
+let r := ByteArray.empty
+let r := r.push x.toUInt8
+let r := r.push (x+1).toUInt8
+let r := r.push (x+2).toUInt8
 r
 
 @[noinline] def mkByteArray2 (x : Nat) : ByteArray :=
 mkByteArray1 x
 
 unsafe def tst6 (x : Nat) : ShareCommonT IO Unit := do
-let a := [mkByteArray1 x];
-let b := [mkByteArray2 x];
-let c := [mkByteArray2 (x+1)];
-IO.println a;
-IO.println b;
-IO.println c;
-check $ ptrAddrUnsafe a != ptrAddrUnsafe b;
-check $ ptrAddrUnsafe a != ptrAddrUnsafe c;
-let a ← shareCommonM a;
-let b ← shareCommonM b;
-let c ← shareCommonM c;
-check $ ptrAddrUnsafe a == ptrAddrUnsafe b;
-check $ ptrAddrUnsafe a != ptrAddrUnsafe c;
+let a := [mkByteArray1 x]
+let b := [mkByteArray2 x]
+let c := [mkByteArray2 (x+1)]
+IO.println a
+IO.println b
+IO.println c
+check $ ptrAddrUnsafe a != ptrAddrUnsafe b
+check $ ptrAddrUnsafe a != ptrAddrUnsafe c
+let a ← shareCommonM a
+let b ← shareCommonM b
+let c ← shareCommonM c
+check $ ptrAddrUnsafe a == ptrAddrUnsafe b
+check $ ptrAddrUnsafe a != ptrAddrUnsafe c
 pure ()
 
 #eval (tst6 2).run
