tests/lean/run/DefEqAssignBug.lean
@@ -5,25 +5,23 @@ new_frontend
 open Lean
 open Lean.Meta
 
-def mkArrow (d b : Expr) : Expr := mkForall `_ BinderInfo.default d b
-
 def checkM (x : MetaM Bool) : MetaM Unit :=
 unlessM x $ throwError "check failed"
 
 def tst1 : MetaM Unit := do
-let nat := mkConst `Nat;
-let m1 ← mkFreshExprMVar nat;
-let m2 ← mkFreshExprMVar (mkArrow nat nat);
-withLocalDeclD `x nat $ fun x => do
-  let t := mkApp m2 x;
+let nat := mkConst `Nat
+let m1 ← mkFreshExprMVar nat
+let m2 ← mkFreshExprMVar (← mkArrow nat nat)
+withLocalDeclD `x nat fun x => do
+  let t := mkApp m2 x
   checkM $ isDefEq t m1
 
 def tst2 : MetaM Unit := do
-let nat := mkConst `Nat;
-let m1 ← mkFreshExprMVar nat;
-let m2 ← mkFreshExprMVar (mkArrow nat nat);
-withLocalDeclD `x nat $ fun x => do
-  let t := mkApp m2 x;
+let nat := mkConst `Nat
+let m1 ← mkFreshExprMVar nat
+let m2 ← mkFreshExprMVar (← mkArrow nat nat)
+withLocalDeclD `x nat fun x => do
+  let t := mkApp m2 x
   checkM $ isDefEq m1 t
 
 set_option trace.Meta true
