tests/lean/run/IO_test.lean
@@ -86,25 +86,25 @@ pure ()
 #eval test2
 
 def test3 : IO Unit := do
-let fn3 := "foo3.txt";
-let xs₀ := "abc";
-let xs₁ := "";
-let xs₂ := "hello";
-let xs₃ := "world";
+let fn3 := "foo3.txt"
+let xs₀ := "abc"
+let xs₁ := ""
+let xs₂ := "hello"
+let xs₃ := "world"
 withFile fn3 Mode.write $ fun h => do {
   pure ()
-};
-let ys ← lines fn3;
-IO.println $ repr ys;
-check_eq "1" ys #[];
+}
+let ys ← lines fn3
+IO.println $ repr ys
+check_eq "1" ys #[]
 withFile fn3 Mode.write $ fun h => do
-{ h.putStrLn xs₀;
-  h.putStrLn xs₁;
-  h.putStrLn xs₂;
-  h.putStrLn xs₃ };
-let ys ← lines fn3;
-IO.println $ repr ys;
-check_eq "2" ys #[xs₀, xs₁, xs₂, xs₃];
+  h.putStrLn xs₀
+  h.putStrLn xs₁
+  h.putStrLn xs₂
+  h.putStrLn xs₃
+let ys ← lines fn3
+IO.println $ repr ys
+check_eq "2" ys #[xs₀, xs₁, xs₂, xs₃]
 pure ()
 
 #eval test3
