tests/lean/run/dofun_prec.lean
@@ -2,7 +2,7 @@ new_frontend
 
 def tst1 (x : Nat) : IO Unit :=
 when (x > 0) do
-  IO.println "hello";
+  IO.println "hello"
   IO.println "world"
 
 def tst2 (xs : List Nat) : IO Unit :=
