tests/lean/run/new_frontend2.lean
@@ -18,29 +18,28 @@ variable [r : Monad m]
 because `Monad.to* methods have bad binder annotations
 -/
 
-theorem aux (a b c : Nat) (h₁ : a = b) (h₂ : c = b) : a = c :=
-by {
-  let! aux := h₂.symm;
-  subst aux;
-  subst h₁;
-  exact rfl
-}
+theorem aux (a b c : Nat) (h₁ : a = b) (h₂ : c = b) : a = c := by
+let! aux := h₂.symm
+subst aux
+subst h₁
+exact rfl
+
 
 def ex1 : {α : Type} → {a b c : α} → a = b → b = c → a = c :=
-@(by intro α a b c h₁ h₂;
+@(by intro α a b c h₁ h₂
      exact Eq.trans h₁ h₂)
 
 def f1 (x : Nat) : Nat := by
-apply (· + ?hole);
-exact 1;
+apply (· + ?hole)
+exact 1
 case hole => exact x
 
 theorem ex2 (x : Nat) : f1 x = 1 + x :=
 rfl
 
 def f2 (x : Nat) : Nat := by
-apply Nat.add _;
-exact 1;
+apply Nat.add _
+exact 1
 exact x
 
 theorem ex3 (x : Nat) : f2 x = x + 1 :=
