tests/lean/run/obtain.lean
@@ -11,15 +11,13 @@ theorem tst2 {p q r} (h : p ∧ q ∧ r) : q ∧ p ∧ r :=
 obtain ⟨h₁, ⟨h₂, h₃⟩⟩ from h;
 ⟨h₂, ⟨h₁, h₃⟩⟩
 
-macro "obtain " p:term " from " d:term "; " body:tactic : tactic =>
-`(tactic| match $d:term with | $p:term => _; $body)
+macro "obtain " p:term " from " d:term : tactic =>
+`(tactic| match $d:term with | $p:term => ?hole)
 
-theorem tst3 {p q r} (h : p ∧ q ∧ r) : q ∧ p ∧ r :=
-by {
-  obtain ⟨h₁, ⟨h₂, h₃⟩⟩ from h;
-  apply And.intro;
-  assumption;
-  apply And.intro;
-  assumption;
+theorem tst3 {p q r} (h : p ∧ q ∧ r) : q ∧ p ∧ r := by
+  obtain ⟨h₁, ⟨h₂, h₃⟩⟩ from h
+  apply And.intro
   assumption
-}
+  apply And.intro
+  assumption
+  assumption
