tests/lean/run/partial1.lean
@@ -3,7 +3,7 @@ new_frontend
 partial def reverse {α} (as : List α) : List α :=
 let rec loop : List α → List α → List α
   | [],    r => r
-  | a::as, r => loop as (a::r);
+  | a::as, r => loop as (a::r)
 loop as []
 
 #eval reverse [3, 2, 1]
@@ -16,7 +16,7 @@ partial def appendRev {α} (extra : List α) (as : List α) : List α :=
 let rec loop (as acc : List α) : List α :=
   match as, acc with
   | [],    r => extra ++ r
-  | a::as, r => loop as (a::r);
+  | a::as, r => loop as (a::r)
 loop as []
 
 #eval appendRev [3, 4] [1, 2, 0]
