tests/lean/run/quasi_pattern_unification_approx_issue.lean
@@ -9,5 +9,5 @@ def foo1 : StateT δ (StateT σ Id) σ :=
 monadLift (get : StateT σ Id σ)
 
 def foo2 : StateT δ (StateT σ Id) σ := do
-let s : σ  ← monadLift (get : StateT σ Id σ);
+let s : σ  ← monadLift (get : StateT σ Id σ)
 pure s
