tests/lean/run/readerThe.lean
@@ -4,17 +4,17 @@ abbrev M := ReaderT String $ StateT Nat $ ReaderT Bool $ IO
 
 
 def f : M Nat := do
-let s ← read;
-IO.println s;
-let b ← readThe Bool;
-IO.println b;
-let s ← get;
+let s ← read
+IO.println s
+let b ← readThe Bool
+IO.println b
+let s ← get
 pure s
 
 #eval (f "hello").run' 10 true
 
 def g : M Nat :=
-let a : M Nat := adaptTheReader Bool not f;
+let a : M Nat := adaptTheReader Bool not f
 adaptReader (fun s => s ++ " world") a
 
 #eval (g "hello").run' 10 true
