tests/lean/run/scc.lean
@@ -3,8 +3,8 @@ new_frontend
 open Lean.SCC
 
 def checkSCC (expected : List (List Nat)) (vertices : List Nat) (successorsOf : Nat → List Nat) : IO Unit := do
-let r := scc vertices successorsOf;
-IO.println r;
+let r := scc vertices successorsOf
+IO.println r
 unless (expected == r) $
   throw $ IO.userError ("expected result " ++ toString expected)
 
