tests/lean/run/spec_issue.lean
@@ -2,6 +2,6 @@ new_frontend
 set_option trace.compiler.ir.result true
 
 def g (ys : List Nat) : IO Nat := do
-let x := 0;
-let (_, x) ← StateT.run (ys.forM fun y => IO.println y) x;
+let x := 0
+let (_, x) ← StateT.run (ys.forM fun y => IO.println y) x
 pure x
