tests/lean/run/stateRef.lean
@@ -1,32 +1,31 @@
 new_frontend
 
 def f (v : Nat) : StateRefT Nat IO Nat := do
-IO.println "hello";
-modify fun s => s - v;
+IO.println "hello"
+modify fun s => s - v
 get
 
 def g : IO Nat :=
-(f 5).run' 20
+f 5 $.run' 20
 
 #eval (f 5).run' 20
 
 #eval (do set 100; f 5 : StateRefT Nat IO Nat).run' 0
-
 def f2 : ReaderT Nat (StateRefT Nat IO) Nat := do
-let v ← read;
-IO.println $ "context " ++ toString v;
-modify fun s => s + v;
+let v ← read
+IO.println $ "context " ++ toString v
+modify fun s => s + v
 get
 
 #eval (f2.run 10).run' 20
 
 def f3 : StateT String (StateRefT Nat IO) Nat := do
-let s ← get;
-let n ← getThe Nat;
-set (s ++ ", " ++ toString n);
-let s ← get;
-IO.println s;
-set (n+1);
+let s ← get
+let n ← getThe Nat
+set $ s ++ ", " ++ toString n
+let s ← get
+IO.println s
+set (n+1)
 getThe Nat
 
 #eval (f3.run' "test").run' 10
@@ -38,31 +37,31 @@ class HasGetAt {β : Type} (v : β) (α : outParam Type) (m : Type → Type) :=
 (getAt : m α)
 
 instance monadState.hasGetAt (β : Type) (v : β) (α : Type) (m : Type → Type) [Monad m] [MonadStateOf (Label v α) m] : HasGetAt v α m :=
-{ getAt := do let a ← getThe (Label v α); pure a.val }
+{ getAt := do let a ← getThe (Label v α); return a.val }
 
 export HasGetAt (getAt)
 
 abbrev M := StateRefT (Label 0 Nat) $ StateRefT (Label 1 Nat) $ StateRefT (Label 2 Nat) IO
 
 def f4 : M Nat := do
-let a0 : Nat ← getAt 0;
-let a1 ← getAt 1;
-let a2 ← getAt 2;
-IO.println $ "state0 " ++ toString a0;
-IO.println $ "state1 " ++ toString a1;
-IO.println $ "state1 " ++ toString a2;
-pure (a0 + a1 + a2)
+let a0 : Nat ← getAt 0
+let a1 ← getAt 1
+let a2 ← getAt 2
+IO.println $ "state0 " ++ toString a0
+IO.println $ "state1 " ++ toString a1
+IO.println $ "state1 " ++ toString a2
+return a0 + a1 + a2
 
-#eval ((f4.run' ⟨10⟩).run' ⟨20⟩).run' ⟨30⟩
+#eval f4.run' ⟨10⟩ $.run' ⟨20⟩ $.run' ⟨30⟩
 
 abbrev S (ω : Type) := StateRefT Nat $ StateRefT String $ ST ω
 
 def f5 {ω} : S ω Unit := do
-let s ← getThe String;
-modify fun n => n + s.length;
+let s ← getThe String
+modify fun n => n + s.length
 pure ()
 
 def f5Pure (n : Nat) (s : String) :=
-runST (fun _ => (f5.run n).run s)
+runST fun _ => f5.run n $.run s
 
 #eval f5Pure 10 "hello world"
